feat: added a strange and fucked up half of a proof lol

lfea/Lfea/Proofs/Regular.lean
@@ -42,7 +42,7 @@ def Dfa.extendedProgram : Dfa σ n → Fin n → List σ → Fin n
   | dfa, q, []        => q
   | dfa, q, (x :: xs) => extendedProgram dfa (dfa.program q x) xs
 
-structure IsAccepted (lang: List σ) (dfa: Dfa σ n) where
+structure Dfa.Accepts (lang: List σ) (dfa: Dfa σ n) where
   proof : (Dfa.extendedProgram dfa dfa.state lang) ∈ dfa.final
 
 inductive Alpha where
@@ -56,7 +56,7 @@ def prog : Fin 4 -> Alpha -> Fin 4
   | 2, Alpha.a => 2
   | _, _ => 3
 
-example : IsAccepted [Alpha.a, Alpha.b] { state := 0, program := prog, final := {x | x == 2}} :=
+example : Dfa.Accepts [Alpha.a, Alpha.b] { state := 0, program := prog, final := {x | x = 2}} :=
     { proof := by simp [Dfa.extendedProgram, Set.in] }
 
 -- NFA
@@ -69,8 +69,14 @@ structure Nfa (sigma: Type) (n: Nat) where
 
 def Nfa.extendedProgram : Nfa σ n → Set (Fin n) → List σ → Set (Fin n)
   | nfa, qs, []        => qs
-  | nfa, qs, (x :: xs) => Set.bigUnion
-    { el | ∃q, q ∈ qs ∧ (el = extendedProgram nfa (nfa.program q x) xs) }
+  | nfa, qs, (x :: xs) => 
+    -- Its a confusing definition
+    -- The result of the extended program is the 
+    -- Big union of all the 
+    Set.bigUnion { el | ∃q, q ∈ qs ∧ (el = extendedProgram nfa (nfa.program q x) xs) }
+
+structure Nfa.Accepts (lang: List σ) (nfa: Nfa σ n) where
+  proof : ∃q, q ∈ (Nfa.extendedProgram nfa {x | x = nfa.state} lang) ∧ q ∈ nfa.final
 
 -- Denotational semantics of Regex
 
@@ -78,5 +84,158 @@ inductive Regex (σ: Type) where
   | var   : σ       -> Regex σ
   | alt   : Regex σ -> Regex σ -> Regex σ
   | conc  : Regex σ -> Regex σ -> Regex σ
-  | plus  : Regex σ -> Regex σ
+  | star  : Regex σ -> Regex σ
   | empty : Regex σ
+
+
+def sizeOfRegex : Regex σ -> Nat
+  | Regex.var _     => 1
+  | Regex.alt a b   => sizeOfRegex a + sizeOfRegex b
+  | Regex.conc a b  => sizeOfRegex a + sizeOfRegex b
+  | Regex.star _    => 1
+  | Regex.empty     => 2
+
+inductive Regex.Accepts : List σ → Regex σ → Type where
+  | acceptsEmpty : Accepts [] Regex.empty
+  | acceptsVar   : Accepts [x] (Regex.var x)
+  | acceptsAltL  : Accepts x l → Accepts x (Regex.alt l r)
+  | acceptsAltR  : Accepts x r → Accepts x (Regex.alt l r)
+  | acceptsConc  : Accepts x a → Accepts y b → Accepts (x ++ y) (Regex.conc a b)
+  | acceptsStar  : Accepts [] (Regex.star a)
+  | acceptsStar2 : Accepts x a → Accepts y (Regex.star a) → Accepts (x ++ y) (Regex.star a)
+
+theorem Regex.NotMatchesEmpty: ∀ {x : σ} {xs : List σ}, Regex.Accepts (x :: xs) Regex.empty → False
+  | x, xs, accepts =>
+    accepts.casesOn
+      (motive := λacc regex proof => (acc = (x :: xs) -> regex = Regex.empty -> False))
+      (λproof _ => List.noConfusion proof) -- acceptsEmpty
+      (λproof ot => Regex.noConfusion ot) -- acceptsVar
+      (λ_ _ ot => Regex.noConfusion ot) -- acceptsAltL
+      (λ_ _ ot => Regex.noConfusion ot) -- acceptsAltR
+      (λ_ _ _ ot => Regex.noConfusion ot) -- acceptsConc
+      (λ _ ot => Regex.noConfusion ot) -- acceptsStar
+      (λ_ _ _ ot => Regex.noConfusion ot) -- acceptsStar2
+      rfl
+      rfl
+
+example : Regex.Accepts ['a', 'a', 'b'] (Regex.conc (Regex.star (Regex.var 'a')) (Regex.var 'b')) :=
+  Regex.Accepts.acceptsConc
+    (Regex.Accepts.acceptsStar2
+      Regex.Accepts.acceptsVar
+      (Regex.Accepts.acceptsStar2
+        Regex.Accepts.acceptsVar
+        Regex.Accepts.acceptsStar))
+    Regex.Accepts.acceptsVar
+
+-- iff redefined lol
+
+structure IIff (a: Type u) (b: Type u) where
+  to : a -> b
+  mpr: b -> a
+
+notation:40 a "`↔" b:40 => IIff a b
+
+universe u
+
+axiom IIff.toEql : ∀ {a b: Type u} (_: IIff a b), a = b
+
+-- ENFA
+
+def Nfa.Nfa_ε.End: Set (Fin 2) := { x | x = 1 }
+
+
+
+def Nfa.Nfa_ε.Final: Fin 2 → Prop := { x | x = 0 }
+
+def Nfa.Nfa_ε : Nfa σ 2 := { state := 0, program := λ _ _ => Nfa.Nfa_ε.End, final := { x | x = 0 }}
+
+def Nfa.Nfa_ε.initial: ∀ {σ: Type}, Set (Fin 2) | x => {y | y = (@Nfa.state x 2 Nfa.Nfa_ε)}
+
+
+theorem Nfa.Nfa_ε.EverythingLeadToEnd : ∀ {q: (Fin 2)} {x: σ}, (Nfa.Nfa_ε.program q x) = Nfa.Nfa_ε.End := by simp; rfl
+
+theorem Nfa.Nfa_ε.EverythingToFinal : ∀ {xs: List σ}, (Nfa.extendedProgram Nfa.Nfa_ε Nfa.Nfa_ε.End xs) = Nfa.Nfa_ε.End
+  | [] => by simp [Nfa.extendedProgram]
+  | (x :: xs) => by
+    simp [Nfa.extendedProgram, Set.bigUnion, Set.subset, Set.in]
+    apply Set.Eq
+    . intro x1
+      simp [Set.in]
+      intro ex
+      apply Exists.elim
+      . assumption
+      . intro state proof
+        simp [Set.in]
+        apply Exists.elim
+        . exact (And.right proof)
+        . intro ata
+          rw [Nfa.Nfa_ε.EverythingLeadToEnd, EverythingToFinal]
+          intro wot
+          rw [←wot.right]
+          exact proof.left
+    . simp [Nfa.extendedProgram, Set.bigUnion, Set.subset, Set.in]
+      intro x1 end_x1
+      exists End
+      apply And.intro
+      . assumption
+      . exact ⟨1, by
+          simp [End]
+          rw [Nfa.Nfa_ε.EverythingLeadToEnd, EverythingToFinal]
+          rfl⟩
+
+theorem Nfa.Nfa_ε.LeadToFinal: ∀ {σ: Type} {x : σ} {xs: List σ}, (Nfa.extendedProgram Nfa.Nfa_ε (@Nfa.Nfa_ε.initial σ) (x :: xs)) = Nfa.Nfa_ε.End
+  | sigm, x, xs => by
+    simp [extendedProgram, Nfa.Nfa_ε.EverythingToFinal, Set.bigUnion, Set.in]
+    apply Set.Eq
+    . simp [Set.in, Set.subset]
+      intro x ex
+      apply Exists.elim
+      . assumption
+      . intro a p
+        apply Exists.elim
+        . exact p.right
+        . intro b
+          rw [Nfa.Nfa_ε.EverythingLeadToEnd, EverythingToFinal]
+          intro f
+          rw [←f.right]
+          exact p.left
+    . simp [Nfa.extendedProgram, Set.bigUnion, Set.subset, Set.in]
+      intro x1 end_x1
+      exists End
+      apply And.intro
+      . assumption
+      . exact ⟨0, And.intro rfl (by rw [Nfa.Nfa_ε.EverythingLeadToEnd, Nfa.Nfa_ε.EverythingToFinal])⟩
+
+theorem Nfa.Nfa_ε.NotAcceptsEntries: ∀ {σ: Type} {x : σ} {xs: List σ}, Nfa.Accepts (x :: xs) Nfa.Nfa_ε → False
+  | sig, x, xs, p => absurd p.proof $ by
+    let f : fun y => y = (@Nfa.state sig 2 Nfa.Nfa_ε) = (@Nfa.Nfa_ε.initial sig) := rfl
+    simp [Set.in,  Nfa.Nfa_ε.LeadToFinal]
+    intro x2
+    apply Exists.elim
+    . assumption
+    . intro a
+      rw [f, Nfa.Nfa_ε.LeadToFinal]
+      simp [End, Nfa_ε]
+      intro and
+      let f := Eq.trans (Eq.symm and.left) and.right
+      contradiction
+
+def toNFA : ∀ (s: List σ), (r: Regex σ) → ∃ (n : Nat), ∃ (e: Nfa σ n), (Regex.Accepts s r) = (Nfa.Accepts s e)
+  | s, Regex.empty =>
+    let iffRes : (s: List σ) → (Regex.Accepts s Regex.empty) `↔ (Nfa.Accepts s Nfa.Nfa_ε)
+      | [] => {
+          to  := by
+            intro a
+            simp [Nfa.Nfa_ε, Nfa.Accepts]
+            exact { proof := by simp [Nfa.extendedProgram]; exact ⟨0, rfl⟩ }
+          mpr := λ _ => Regex.Accepts.acceptsEmpty
+        }
+      | (x :: xs) => {
+        to := λ x => False.elim (Regex.NotMatchesEmpty x)
+        mpr := λx => False.elim (Nfa.Nfa_ε.NotAcceptsEntries x)
+      }
+    ⟨2, ⟨Nfa.Nfa_ε, IIff.toEql (iffRes s)⟩⟩
+  | s, Regex.var a     => sorry
+  | s, Regex.star a    => sorry
+  | s, Regex.conc a b  => sorry
+  | s, Regex.alt a b   => sorry
